backend/Unusedglobproof.v
@@ -50,6 +50,7 @@ Class MemoryModelX (mem: Type) `{memory_model_prf: MemoryModel mem}: Prop :=
        exists v2,
          loadbytes m2 b2 o 1 = Some (v2 :: nil) /\
          memval_inject f v1 v2) ->
+  list_forall2 (frame_inject f m1) (stack_adt m1) (stack_adt m2) ->
   inject f m1 m2
 }.
 
@@ -1105,7 +1106,17 @@ Proof.
     intros. destruct (eq_block b1 stk).
     subst b1. rewrite F in H2; inv H2. split; apply Ple_refl.
     rewrite G in H2 by auto. congruence. }
-  exploit Mem.record_stack_block_inject; eauto. intros (m2' & RSB & INJ).
+  exploit Mem.record_stack_block_inject; eauto.
+  eapply Mem.frame_inject_with_info.
+  {
+   rewrite F. inversion 1; subst; auto. 
+  }
+  {
+    intros b' delta.
+    destruct (eq_block b' stk); auto. rewrite G; inversion 1; auto.
+    eapply Mem.valid_block_inject_2 in H1; eauto. eapply Mem.fresh_block_alloc in H1; eauto. easy.
+  }
+  intros (m2' & RSB & INJ).
   econstructor; split.
   eapply exec_function_internal; eauto.
   eapply match_states_regular with (j := j'); eauto.
@@ -1173,6 +1184,87 @@ Proof.
   exploit defs_inject. apply init_meminj_preserves_globals.
   eauto. eauto. intros (X & _ & Y). 
   eauto.
+Qed.
+
+Lemma store_init_data_stack_adt:
+  forall {F V} l (ge: Genv.t F V) m m' b ofs,
+    Genv.store_init_data ge m b ofs l = Some m' ->
+    Mem.stack_adt m' = Mem.stack_adt m.
+Proof.
+  destruct l; simpl; intros;
+  try now (eapply Mem.store_stack_blocks; eauto).
+  inv H; auto.
+  destruct (Genv.find_symbol ge0 i); try discriminate.  
+  eapply Mem.store_stack_blocks; eauto.
+Qed.
+
+Lemma store_init_data_list_stack_adt:
+  forall {F V} l (ge: Genv.t F V) m m' b ofs,
+    Genv.store_init_data_list ge m b ofs l = Some m' ->
+    Mem.stack_adt m' = Mem.stack_adt m.
+Proof.
+  induction l; simpl; intros; eauto.
+  inv H; auto.
+  destruct Genv.store_init_data eqn:?; try discriminate.
+  erewrite IHl. 2: eauto.
+  eapply store_init_data_stack_adt; eauto.
+Qed.
+
+Lemma store_zeros_stack_adt:
+  forall m b lo hi m',
+    store_zeros m b lo hi = Some m' ->
+    Mem.stack_adt m' = Mem.stack_adt m.
+Proof.
+  intros.
+  revert H.
+  eapply store_zeros_ind; simpl; intros.
+  inv H; auto.
+  erewrite H, Mem.store_stack_blocks; eauto.
+  inv H. 
+Qed.
+
+Lemma alloc_global_stack_adt:
+  forall {F V} l (ge: Genv.t F V) m m',
+    Genv.alloc_global ge m l = Some m' ->
+    Mem.stack_adt m' = Mem.stack_adt m.
+Proof.
+  destruct l; simpl; intros.
+  destruct o. destruct g.
+  destruct (Mem.alloc m 0 1) eqn:?; try discriminate.
+  erewrite Mem.drop_perm_stack_adt. 2: eauto.
+  eapply Mem.alloc_stack_blocks; eauto.
+  destruct (Mem.alloc m 0 (init_data_list_size (gvar_init v))) eqn:?.
+  destruct store_zeros eqn:?; try discriminate.
+  destruct Genv.store_init_data_list eqn:?; try discriminate.
+  erewrite Mem.drop_perm_stack_adt. 2: eauto.
+  erewrite store_init_data_list_stack_adt. 2: eauto.
+  erewrite store_zeros_stack_adt. 2: eauto.
+  eapply Mem.alloc_stack_blocks; eauto.
+  destruct Mem.alloc eqn:?.
+  inv H.
+  eapply Mem.alloc_stack_blocks; eauto.
+Qed.
+
+Lemma alloc_globals_stack_adt:
+  forall {F V} l (ge: Genv.t F V) m m',
+    Genv.alloc_globals ge m l = Some m' ->
+    Mem.stack_adt m' = Mem.stack_adt m.
+Proof.
+  induction l; simpl; intros; eauto. congruence.
+  destruct (Genv.alloc_global ge0 m a) eqn:?; try discriminate.
+  erewrite IHl. 2: eauto. 
+  eapply alloc_global_stack_adt; eauto.
+Qed.
+
+Lemma init_mem_stack_adt:
+  forall {F V} (p: AST.program F V) m,
+    Genv.init_mem p = Some m ->
+    Mem.stack_adt m = nil.
+Proof.
+  unfold Genv.init_mem.
+  intros.
+  erewrite alloc_globals_stack_adt; eauto.
+  eapply Mem.empty_stack_adt.
 Qed.
 
 Section INIT_MEM.
@@ -1364,6 +1456,10 @@ Proof.
   edestruct GINIT; eauto.
   eapply H0.
   instantiate (1 := o); omega.
+- 
+  rewrite (init_mem_stack_adt _ _ IM).
+  rewrite (init_mem_stack_adt _ _ TIM).
+  constructor.
 (*
   destruct gd as [f|v].
 + intros (P2 & Q2) (P1 & Q1).
